

Two Pages on Logistic Regression

Mathias Winther Madsen

January 31, 2025

The inverse of the **logistic function**

$$\log \frac{p}{1-p} \quad (0 < p < 1)$$

is the **sigmoid function**

$$\begin{aligned}\sigma(t) &= \frac{1}{1+e^{-t}} = \frac{e^t}{e^t+1} \\ \sigma'(t) &= \frac{e^{-t}}{(1+e^{-t})^2} = \sigma(t)\sigma(-t)\end{aligned}$$

Its logarithm satisfies

$$\begin{aligned}\log \sigma(t) &= \log(1+e^{-t}) \\ \log \sigma(t)' &= \sigma(-t)\end{aligned}$$

The sigmoid function is perfectly anti-symmetric around zero in the sense that

$$\underbrace{\sigma(t)}_p + \underbrace{\sigma(-t)}_{1-p} = 1.$$

It is therefore a good choice for relating a scalar evidence variable t to the probabilities of two exclusive possibilities, say, $y = +1$ or $y = -1$.

In logistic regression, we assume that the posterior log-odds in favor of some positive hypothesis is an affine function of some feature vector x :

$$u = \log \frac{p(+1|x)}{p(-1|x)} = a^T x + b.$$

This implies that

$$\begin{aligned}p(+1|x) &= \sigma(+u) \\ p(-1|x) &= \sigma(-u)\end{aligned}$$

Hence if $y \in \{-1, +1\}$ is the true state of affairs, then $\sigma(yu)$ is the posterior probability assigned to the correct hypothesis. Under the logarithmic scoring rule for probability assignments, the model's loss at observing (x, y) is then

$$-\log \sigma(yu).$$

For notational convenience, we can define the vectors $w = (a \ b)$ and $z = y(x \ 1)$. We then get following formulas for the resulting loss function:

$$\begin{aligned} L(w) &= - \sum_n \log \sigma(w^T z_n) \\ \nabla_w L(w) &= - \sum_n \sigma(-w^T z_n) z_n \\ \nabla_w^2 L(w) &= + \sum_n \sigma(w^T z_n) \sigma(-w^T z_n) z_n z_n^T \end{aligned}$$

We can optimize this objective function using Newton's method, which here takes the form of the update rule

$$w_{i+1} = w_i - (\nabla_w^2 L(w_i))^{-1} (\nabla_w L(w_i)).$$